theories/iris/logrel/function.v
@@ -1,0 +1,46 @@
+From iris.proofmode Require Export base proofmode classes.
+
+From RichWasm Require Import syntax typing.
+From RichWasm.compiler Require Import prelude module.
+Require Import RichWasm.iris.host.iris_host.
+Require Import RichWasm.iris.rules.iris_rules.
+From RichWasm.iris Require Import logrel memory util.
+
+Module W := RichWasm.wasm.datatypes.
+
+Set Bullet Behavior "Strict Subproofs".
+Set Default Goal Selector "!".
+
+Section function.
+
+  Context `{!logrel_na_invs Σ}.
+  Context `{!wasmG Σ}.
+  Context `{!richwasmG Σ}.
+
+  Variable rti : rt_invariant Σ.
+  Variable sr : store_runtime.
+
+  Theorem fundamental_function mr M wt wt' wtf mf mf' ϕ :
+    has_function_type M mf ϕ ->
+    compile_function wt mf = inr (wt', mf') ->
+    ⊢ has_func_type_sem rti sr mr M (wt ++ wt' ++ wtf) mf' ϕ.
+  Proof.
+    iIntros (Hϕ Hcf ?? Htf) "#Hinst".
+    inversion Hϕ.
+    subst M0 mf0 ϕ ϕ0 ϕ1.
+    set (ϕ := mf.(mf_type)) in *.
+    set (fft := flatten_function_type ϕ) in *.
+    rename H into Hηss_L.
+    rename H0 into Hρs_P.
+    rename H1 into Hηss_P.
+    rename H3 into Hψ.
+    rename H2 into HL'.
+    destruct tf as [ts1 ts2].
+    rewrite closure_interp_eq.
+
+    (* TODO: By induction on ϕ, build up an se such that sem_env_interp F se.
+             Then use the fundamental theorem for instruction typing to show that the body of the
+             function is well-behaved. *)
+  Admitted.
+
+End function.
